

## Lecture-1

### Background Information

**Abstract:** In this lecture we provide background information needed to study the subjects of Analog Communication course.

### Impulse or Dirac delta function

Continuous time impulse function is defined as

$$\delta(t) = \begin{cases} 0 & t \neq 0 \\ \infty & t = 0 \end{cases} \quad \text{and we have} \quad \int_{-\infty}^{\infty} \delta(t) dt = 1.$$

The impulse function satisfies the properties

a)

$$g(t)\delta(t - t_0) = g(t_0)\delta(t - t_0)$$

$$g(t - t_1)\delta(t - t_0) = g(t_0 - t_1)\delta(t - t_0)$$

b)

$$\int_{-\infty}^{\infty} g(t)\delta(t - t_0) dt = g(t_0)$$

c)

$$\int_{-\infty}^{\infty} g(t - t_1)\delta(t - t_0) dt = g(t_0 - t_1)$$

d)

$$\delta(a(t - t_0)) = \frac{1}{|a|} \delta(t - t_0)$$

$$\delta(at) = \frac{1}{|a|} \delta(t)$$

e)

$$g(t) * \delta(t - t_0) = g(t - t_0)$$

$$g(t - t_1) * \delta(t - t_0) = g(t - t_0 - t_1)$$

where  $*$  denotes the convolution operation.

### Complex Exponential Function

The complex exponential function  $e^{j\theta}$  is defined as

$$e^{j\theta} = \cos \theta + j \sin \theta.$$

The function  $e^{j\theta}$  satisfies the property

$$|e^{j\theta}| = 1$$

since we have

$$|e^{j\theta}| = |\cos \theta + j \sin \theta| \rightarrow |e^{j\theta}| = \sqrt{(\cos \theta)^2 + (\sin \theta)^2}$$

Note that the complex number  $a = b + jc$  can be expressed as

$$a = |a|e^{j\angle a}$$

where

$$|a| = \sqrt{b^2 + c^2} \quad \text{and} \quad \angle a = \arctan \frac{c}{b}.$$

**Example:** Calculate  $\angle e^{j\theta}$ .

**Solution:** The expression  $\angle e^{j\theta}$  can be written as

$$e^{j\theta} = \cos \theta + j \sin \theta$$

whose phase can be calculated as

$$\angle e^{j\theta} = \tan^{-1} \frac{\sin \theta}{\cos \theta} \rightarrow \angle e^{j\theta} = \tan^{-1} \frac{\sin \theta}{\cos \theta}$$

leading to

$$\angle e^{j\theta} = \tan^{-1} \tan \theta \rightarrow \angle e^{j\theta} = \theta.$$

Note that if  $f(x)$  is a function and  $f^{-1}(x)$  is the inverse function, then we have the property,

$$f^{-1}(f(x)) = x \quad \text{or} \quad f(f^{-1}(x)) = x.$$

**Example:** Write  $\cos(\theta)$  in terms of the complex exponential functions.

**Solution:** We can write  $e^{j\theta}$  and  $e^{-j\theta}$  as in

$$e^{j\theta} = \cos \theta + j \sin \theta \quad (A)$$

$$e^{-j\theta} = \cos \theta - j \sin \theta \quad (B)$$

Summing (A) and (B), we obtain

$$e^{j\theta} + e^{-j\theta} = \cos \theta + j \sin \theta + \cos \theta - j \sin \theta$$

from which we get

$$\cos \theta = \frac{1}{2}(e^{j\theta} + e^{-j\theta}).$$

**Exercise:** Show that  $\sin \theta$  can be written as

$$\sin \theta = \frac{1}{2j}(e^{j\theta} - e^{-j\theta})$$

### Unit Step Function

The unit step function can be defined either as

$$u(t) = \begin{cases} 1 & t \geq 0 \\ 0 & \text{otherwise} \end{cases}$$

or as

$$u(t) = \begin{cases} 1 & t > 0 \\ \frac{1}{2} & t = 0 \\ 0 & \text{otherwise.} \end{cases}$$

The relation between impulse function and unit step function can be expressed as

$$\delta(t) = \frac{du(t)}{dt}$$

$$u(t) = \int_{-\infty}^t \delta(t) dt.$$

## Continuous Time Fourier Transform

The Fourier transform of the continuous time signal  $g(t)$  is calculated as

$$G(w) = \int_{-\infty}^{\infty} g(t)e^{-j\omega t} dt \quad (1)$$

where  $w$  is the angular frequency and  $j$  is the complex number such that  $j = \sqrt{-1}$ .

Employing  $w = 2\pi f$  in (1), we can express the Fourier transform of  $g(t)$  as in

$$G(2\pi f) = \int_{-\infty}^{\infty} g(t)e^{-j2\pi ft} dt \rightarrow G(f) = \int_{-\infty}^{\infty} g(t)e^{-j2\pi ft} dt$$

**Note that**

$$w = 2\pi f$$

is the angular frequency, and its unit is radian/sec. On the other hand the unit of the  $f$  is *Hertz*, i.e., *Hz*, and we have

$$1 \text{ Hz} = \frac{1}{1 \text{ sec}}.$$

## Inverse Fourier Transform

The inverse Fourier transform of  $G(w)$  is defined as

$$g(t) = \frac{1}{2\pi} \int_{-\infty}^{\infty} G(w)e^{j\omega t} d\omega \quad (2)$$

where  $w$  is the angular frequency and  $j$  is the complex number such that  $j = \sqrt{-1}$ .

If we use  $w = 2\pi f$  in (2), we obtain

$$g(t) = \frac{1}{2\pi} \int_{-\infty}^{\infty} G(2\pi f)e^{j2\pi ft} 2\pi df \rightarrow g(t) = \int_{-\infty}^{\infty} G(f)e^{j2\pi ft} df.$$

In brief, Fourier transform and inverse Fourier transform formulas for the signal  $g(t)$  can be written as

$$G(f) = \int_{-\infty}^{\infty} g(t)e^{-j2\pi ft} dt$$

and

$$g(t) = \int_{-\infty}^{\infty} G(f) e^{j2\pi ft} df$$

respectively.

The Fourier transform function  $G(f)$  is a complex function, and it can be expressed as

$$G(f) = |G(f)| e^{j\theta(f)} \quad (3)$$

where  $|G(f)|$  is called magnitude spectrum of  $g(t)$  and  $\theta(f)$  is called phase spectrum of  $g(t)$ .

$G(f)$  can also be written as

$$G(f) = X(f) + jY(f) \quad (4)$$

Using (3) and (4) we can write

$$|G(f)| = \sqrt{X^2(f) + Y^2(f)} \quad \theta(f) = \arctan \frac{Y(f)}{X(f)}.$$

**Example:** The Fourier transform of a continuous function is given as

$$G(f) = \frac{1}{1 - jf}$$

Find  $|G(f)|$  and  $\theta(f)$ .

**Solution:** The Fourier transform expression can be written as

$$G(f) = \frac{1}{1 + j2f} \rightarrow G(f) = \frac{1}{1 + 4f^2} - j \frac{2f}{1 + 4f^2}$$

We calculate the magnitude and phase spectrums as

$$|G(f)| = \sqrt{\frac{1}{(1 + 4f^2)^2} + \frac{4f^2}{(1 + 4f^2)^2}} \rightarrow$$

$$|G(f)| = \sqrt{\frac{1}{1 + 4f^2}}$$

$$\theta(f) = \arctan \frac{\text{Im}[G(f)]}{\text{Real}[G(f)]} \rightarrow \theta(f) = \arctan \frac{-\frac{2f}{1+4f^2}}{\frac{1}{1+4f^2}} \rightarrow \theta(f) = \arctan(-2f)$$

Thus

$$\theta(f) = -\arctan 2f$$

**Example:** Show that

$$\arctan(-x) = -\arctan x$$

.

**Proof:** We know that  $\tan(-x) = -\tan x$ .

If

$$y = \arctan(-x)$$

then we have

$$-x = \tan y$$

from which we get

$$x = \tan(-y)$$

leading to

$$-y = \arctan x$$

which can be written as

$$y = -\arctan x$$

**Example:** Find

$$\angle \cos(\pi f)$$

**Solution:**

**Example:** Given

$$G(f) = 1 + e^{-j2\pi f}$$

find  $|G(f)|$

**Solution:** The complex function

$$G(f) = 1 + e^{-j2\pi f}$$

can be written as

$$G(f) = 1 + e^{-j2\pi f} = 1 + \cos 2\pi f - j \sin 2\pi f$$

and  $|G(f)|$  can be calculated as

$$|G(f)| = \sqrt{(1 + \cos 2\pi f)^2 + (\sin 2\pi f)^2}$$

leading to

$$|G(f)| = \sqrt{1 + 2 \cos 2\pi f + (\cos 2\pi f)^2 + (\sin 2\pi f)^2}$$

where using

$$(\cos 2\pi f)^2 + (\sin 2\pi f)^2 = 1$$

we get

$$|G(f)| = \sqrt{2 + 2 \cos 2\pi f}$$

which can be written as

$$|G(f)| = \sqrt{2} \sqrt{1 + \cos 2\pi f}$$

where using

$$\cos 2\pi f = 2 \cos^2 \pi f - 1$$

we get

$$|G(f)| = 2 |\cos(\pi f)|$$

**Example:** For the given analog signal  $g(t) = \delta(t) + \delta(t - 1)$  find the magnitude and phase spectrum functions.

**Solution:** Using the Fourier transform formula

$$G(f) = \int_{-\infty}^{\infty} g(t) e^{-j2\pi f t} dt$$

for the given function, we obtain

$$G(f) = \int_{-\infty}^{\infty} (\delta(t) + \delta(t - 1)) e^{-j2\pi f t} dt$$

in which using the property

$$\int \delta(t - t_0) f(t) dt = f(t_0)$$

we get

$$G(f) = e^{-j2\pi f 0} + e^{-j2\pi f 1} \rightarrow G(f) = 1 + e^{-j2\pi f} \quad (6)$$

The spectrum expression in (6) can be manipulated as

$$G(f) = 2e^{-j\pi f} \cos(\pi f) \quad (7)$$

From (7), the magnitude and phase spectrums can be calculated as

$$|G(f)| = |2| \underbrace{|e^{-j\pi f}|}_{=1} |\cos(\pi f)| \rightarrow |G(f)| = 2 |\cos(\pi f)|$$

$$\angle G(f) = \angle 2 + \angle e^{-j\pi f} + \angle \cos(\pi f) \rightarrow \angle G(f) = 0 - \pi f + \angle \cos(\pi f)$$

The period of  $\cos(\pi f)$  is 2, and in one period  $\angle \cos(\pi f)$  can be written as

$$\theta_c(f) = \angle \cos(\pi f) = \begin{cases} 0 & f \leq 0.5 \text{ or } 1.5 \leq f < 2 \\ \pi & 0.5 < f < 1.5 \end{cases}$$

$\angle \cos(\pi f)$  can be written as

$$\angle \cos(\pi f) = \sum_k \theta_c(f - k2).$$

### Fourier transform of the complex exponential signal

The Fourier transform of  $e^{jw_0 t}$  is

$$2\pi\delta(w - w_0)$$

i.e., we have the pair

$$e^{jw_0 t} \xleftrightarrow{FT} 2\pi\delta(w - w_0) \quad (8)$$

If we use  $w = 2\pi f$  and  $w_0 = 2\pi f_0$  in (8), we get

$$e^{j2\pi f_0 t} \xleftrightarrow{FT} 2\pi\delta(2\pi f - 2\pi f_0)$$

where the right hand side can be written as

$$2\pi\delta(2\pi f - 2\pi f_0) \rightarrow 2\pi\delta(2\pi(f - f_0)) \quad (9)$$

in which using the property

$$\delta(a(f - f_0)) = \frac{1}{|a|} \delta(f - f_0)$$

we simplify the right hand side of (9) as

$$2\pi\delta(2\pi(f - f_0)) \rightarrow \frac{2\pi}{2\pi} \delta((f - f_0)) \rightarrow \delta(f - f_0).$$

Thus, we have

$$e^{j2\pi f_0 t} \xleftrightarrow{FT} \delta(f - f_0) \quad (10)$$

**Example:** If  $G(f) = \delta(f - f_0)$ , find  $g(t)$  using inverse Fourier transform formula.

**Solution:** Employing the inverse Fourier transform formula



$$g(t) = \int_{-\infty}^{\infty} G(f) e^{j2\pi f t} df$$

for the given Fourier transform we get

$$g(t) = \int_{-\infty}^{\infty} \delta(f - f_0) e^{j2\pi f t} df$$

in which using the property

$$\int \delta(f - f_0) G(f) df = G(f_0)$$

we obtain

$$g(t) = e^{j2\pi f_0 t}$$

which is the complex exponential function.

### Fourier Transforms of Sine and Cosine Functions

The sine and cosine functions  $\sin(2\pi f_0 t)$  and  $\cos(2\pi f_0 t)$  can be written in terms of the complex exponential functions as

$$\sin(2\pi f_0 t) = \frac{1}{2j} (e^{j2\pi f_0 t} - e^{-j2\pi f_0 t})$$

$$\cos(2\pi f_0 t) = \frac{1}{2} (e^{j2\pi f_0 t} + e^{-j2\pi f_0 t})$$

Using (10) we can evaluate the Fourier transforms of the sine and cosine signals as

$$\sin(2\pi f_0 t) \stackrel{FT}{\leftrightarrow} \frac{1}{2j} (\delta(f - f_0) - \delta(f + f_0))$$

$$\cos(2\pi f_0 t) \stackrel{FT}{\leftrightarrow} \frac{1}{2} (\delta(f - f_0) + \delta(f + f_0))$$

### Properties of Fourier Transform

#### Linearity:

Let

$$g_1(t) \stackrel{FT}{\leftrightarrow} G_1(f)$$

$$g_2(t) \xleftrightarrow{FT} G_2(f)$$

then we have

$$ag_1(t) + bg_2(t) \xleftrightarrow{FT} aG_1(f) + bG_2(f).$$

**Time Scaling:**

If

$$g(t) \xleftrightarrow{FT} G(f)$$

then we have

$$g(at) \xleftrightarrow{FT} \frac{1}{|a|} G\left(\frac{f}{a}\right).$$

**Example:** Using

$$\cos(2\pi f_0 t) \xleftrightarrow{FT} \frac{1}{2} (\delta(f - f_0) + \delta(f + f_0))$$

and time scaling property, we can find the Fourier transform of

$$\cos(\pi f_0 t)$$

as

$$\frac{1}{1/2} \frac{1}{2} \left( \delta\left(\frac{f}{1/2} - f_0\right) + \delta\left(\frac{f}{1/2} + f_0\right) \right)$$

which can be written as

$$\delta(2f - f_0) + \delta(2f + f_0)$$

which is written as

$$\delta\left(2\left(f - \frac{f_0}{2}\right)\right) + \delta\left(2\left(f + \frac{f_0}{2}\right)\right)$$

leading to

$$\frac{1}{2} \left[ \delta\left(f - \frac{f_0}{2}\right) + \delta\left(f + \frac{f_0}{2}\right) \right]$$

In fact, writing  $\cos(\pi f_0 t)$  as

$$\cos\left(2\pi \left(\frac{f_0}{2}\right) t\right)$$

and using

$$\cos(2\pi f' t) \xleftrightarrow{FT} \frac{1}{2} (\delta(f - f') + \delta(f + f'))$$

we can get the same result.

### Duality:

If

$$g(t) \stackrel{FT}{\leftrightarrow} G(f)$$

then we have

$$G(t) \stackrel{FT}{\leftrightarrow} g(-f).$$

**Example:** Using

$$\cos(2\pi f_0 t) \stackrel{FT}{\leftrightarrow} \frac{1}{2}(\delta(f - f_0) + \delta(f + f_0))$$

and duality property we can write

$$\frac{1}{2}(\delta(t - t_0) + \delta(t + t_0)) \stackrel{FT}{\leftrightarrow} \cos(2\pi f t_0)$$

### Time Shifting:

If

$$g(t) \stackrel{FT}{\leftrightarrow} G(f)$$

then we have

$$g(t - t_0) \stackrel{FT}{\leftrightarrow} e^{-j2\pi f t_0} G(f).$$

### Frequency Shifting:

If

$$g(t) \stackrel{FT}{\leftrightarrow} G(f)$$

then we have

$$e^{j2\pi f_0 t} g(t) \stackrel{FT}{\leftrightarrow} G(f - f_0).$$

### Differentiation:

If

$$g(t) \stackrel{FT}{\leftrightarrow} G(f)$$

then we have

$$\frac{dg(t)}{dt} \stackrel{FT}{\leftrightarrow} j2\pi f G(f).$$

In general, we have

$$\frac{d^n g(t)}{dt^n} \stackrel{FT}{\leftrightarrow} (j2\pi f)^n G(f).$$

### Convolution in Time Domain

Let

$$g_1(t) \stackrel{FT}{\leftrightarrow} G_1(f)$$

$$g_2(t) \stackrel{FT}{\leftrightarrow} G_2(f)$$

then we have

$$g_1(t) * g_2(t) \stackrel{FT}{\leftrightarrow} G_1(f)G_2(f)$$

where  $*$  denotes the convolution operation.

**Note:**

$$g_1(t) * g_2(t) = \int_{-\infty}^{\infty} g_1(\tau)g_2(t - \tau)d\tau$$

### Convolution in Frequency Domain

Let

$$g_1(t) \stackrel{FT}{\leftrightarrow} G_1(f)$$

$$g_2(t) \stackrel{FT}{\leftrightarrow} G_2(f)$$

then we have

$$g_1(t)g_2(t) \stackrel{FT}{\leftrightarrow} G_1(f) * G_2(f)$$

where  $*$  denotes the convolution operation.

**Note:**

$$G_1(f) * G_2(f) = \int_{-\infty}^{\infty} G_1(\tau)G_2(f - \tau)d\tau$$